update mathlib, "squeeze" simps, style

src/matroid.lean
@@ -6,48 +6,46 @@ import data.finset tactic.wlog data.equiv.list tactic.find
 variables {α : Type*} {β : Type*} [decidable_eq α]
 
 namespace finset
-
+/- For mathlib? -/
 lemma inter_of_subset {A B : finset α} (h : A ⊆ B) : A ∩ B = A :=
-by simp [ext]; exact λ a, iff.intro (λ H, H.1) (λ H, ⟨H, mem_of_subset h H⟩)
+lattice.inf_of_le_left h
 
 lemma subset_iff_sdiff_eq_empty {x y : finset α} : x ⊆ y ↔ x \ y = ∅ :=
-by simp [sdiff_eq_filter, eq_empty_iff_forall_not_mem, subset_iff]
-
-lemma inter_subset_inter_of_subset {x y : finset α} (h₁ : x ⊆ y) (z : finset α) : x ∩ z ⊆ y ∩ z :=
-by simp [subset_iff]; exact λ a h₂ h₃, ⟨h₁ h₂, h₃⟩
+by simp only [sdiff_eq_filter, eq_empty_iff_forall_not_mem, subset_iff, not_and,
+  not_not, finset.mem_filter]
 
 lemma empty_sdiff (E : finset α): E \ ∅ = E :=
-by simp [ext]
+by simp only [ext, finset.not_mem_empty, and_true, iff_self, finset.mem_sdiff,
+  not_false_iff, forall_true_iff]
 
-lemma sdiff_subset (A B : finset α): A \ B ⊆ A := (empty_sdiff A).subst $ sdiff_subset_sdiff (subset.refl A) $ empty_subset B
+lemma sdiff_subset (A B : finset α): A \ B ⊆ A :=
+(empty_sdiff A).subst $ sdiff_subset_sdiff (subset.refl A) $ empty_subset B
 
 lemma sdiff_eq_sdiff_inter (A B : finset α) : A \ B = A \ (A ∩ B) :=
-by simp [ext]; exact λ a, iff.intro (λ h, ⟨h.1, λ x, h.2⟩) (λ h, ⟨h.1, h.2 h.1⟩)
-
-lemma union_eq_union_sdiff (A B : finset α) : A ∪ B = A ∪ (B \ A) :=
-by simp [ext]; exact λ a, ⟨λ ha, or.elim ha (λ H, or.inl H)
-  (by { intro H, by_cases h : a ∈ A, { exact or.inl h }, { exact or.inr ⟨H, h⟩ } }),
-  λ ha, or.elim ha (λ H, or.inl H) (λ H, or.inr H.1)⟩
+by { simp only [ext, not_and, mem_sdiff, mem_inter],
+  exact λ a, iff.intro (λ h, ⟨h.1, λ x, h.2⟩) (λ h, ⟨h.1, h.2 h.1⟩) }
 
 lemma card_eq_inter_sdiff (A B : finset α) : card A = card (A ∩ B) + card (A \ B) :=
 begin
-  have hA : A \ B ∪ A ∩ B = A := by simp [ext];
+  have hA : A \ B ∪ A ∩ B = A := by { simp only [ext, mem_union, union_comm, mem_sdiff, mem_inter],
     exact λ a, iff.intro (λ ha, or.elim ha (λ H, H.1) (λ H, H.1))
-      (by { intro ha, by_cases h : a ∈ B, { exact or.inl ⟨ha, h⟩ }, { exact or.inr ⟨ha, h⟩ } }),
-  have : disjoint (A \ B) (A ∩ B) := by simp [disjoint],
+      (by { intro ha, by_cases h : a ∈ B, { exact or.inl ⟨ha, h⟩ }, { exact or.inr ⟨ha, h⟩ } }) },
+  have : disjoint (A \ B) (A ∩ B) := by simp only [disjoint, empty_subset, inf_eq_inter,
+    inter_empty, sdiff_inter_self, inter_left_comm, le_iff_subset],
   replace this := card_disjoint_union this, rwa [hA, add_comm] at this
 end
 
-lemma card_sdiff (A B : finset α) : card (A \ B) = card A - card (A ∩ B) :=
+lemma card_sdiff_eq (A B : finset α) : card (A \ B) = card A - card (A ∩ B) :=
 (nat.sub_eq_of_eq_add $ card_eq_inter_sdiff A B).symm
 
 lemma card_union_inter (A B : finset α) : card A + card B = card (A ∪ B) + card (A ∩ B) :=
 begin
   have hBA : card B = card (B \ A) + card (A ∩ B) := inter_comm B A ▸
     (add_comm (card (B ∩ A)) (card (B \ A))) ▸ (card_eq_inter_sdiff B A),
-  have Hdis : disjoint A (B \ A) := by simp [disjoint],
+  have Hdis : disjoint A (B \ A) := by simp only [disjoint, empty_subset, inf_eq_inter,
+    inter_sdiff_self, le_iff_subset],
   have H : card A + card (B \ A) = card (A ∪ B) :=
-    (congr_arg card $ union_eq_union_sdiff A B).substr (card_disjoint_union Hdis).symm,
+    (congr_arg card $ union_sdiff_self_eq_union.symm).substr (card_disjoint_union Hdis).symm,
   calc
   card A + card B = card A + card (B \ A) + card (A ∩ B) : by rw [add_assoc, hBA]
   ... = card (A ∪ B) + card (A ∩ B) : by rw H
@@ -55,8 +53,9 @@ end
 
 /- proof by Kenny Lau https://leanprover.zulipchat.com/#narrow/stream/113489-new-members/subject/choosing.20from.20difference.20of.20finsets/near/133624012 -/
 lemma exists_sdiff_of_card_lt {x y : finset α} (hcard : card x < card y) : ∃ e : α, e ∈ y \ x :=
-suffices ∃ e ∈ y, e ∉ x, by simpa,
-by_contradiction $ λ H, not_le_of_lt hcard $ card_le_of_subset $ by simpa using H
+suffices ∃ e ∈ y, e ∉ x, by simpa only [exists_prop, finset.mem_sdiff],
+by_contradiction $ λ H, not_le_of_lt hcard $ card_le_of_subset $ by simpa only [not_exists,
+  exists_prop, not_and, not_not] using H
 
 /- proof by chris hughes
 https://leanprover.zulipchat.com/#narrow/stream/113489-new-members/subject/maximal.20finset.20in.20finset.20of.20finsets/near/133905271 -/
@@ -70,7 +69,7 @@ lemma min_fun_of_ne_empty {F : finset β} (func : β → ℕ) (h : F ≠ ∅) :
   ∃ x ∈ F, ∀ g ∈ F, func x ≤ func g :=
 let ⟨n, hn⟩ := (min_of_ne_empty $ mt image_eq_empty.1 h : ∃ a, a ∈ finset.min (F.image func)) in
 let ⟨x, hx₁, hx₂⟩ := mem_image.1 (mem_of_min hn) in
-  ⟨x, hx₁, hx₂.symm ▸ λ g hg, le_min_of_mem (mem_image.2 ⟨g, hg, rfl⟩) hn⟩
+  ⟨x, hx₁, hx₂.symm ▸ λ g hg, min_le_of_mem (mem_image.2 ⟨g, hg, rfl⟩) hn⟩
 
 section inst
 
@@ -78,10 +77,10 @@ variables {F : finset α} {Q : finset α → Prop} [decidable_pred Q] {P : α �
 
 instance decidable_not_forall (c₁ : finset (finset α)) :
   decidable (∃ x : finset α, ¬(x ∈ c₁ → ¬Q x)) :=
-decidable_of_iff (∃ x ∈ c₁, Q x) $ by simp
+decidable_of_iff (∃ x ∈ c₁, Q x) $ by simp only [exists_prop, not_forall_not]
 
 instance decidable_exists_and_mem : decidable (∃ e, e ∈ F ∧ P e) :=
-decidable_of_iff (∃ e ∈ F, P e) $ by simp
+decidable_of_iff (∃ e ∈ F, P e) $ by simp only [exists_prop, not_forall_not]
 
 end inst
 
@@ -114,7 +113,7 @@ instance indep_repr [has_repr α] (E : finset α) : has_repr (indep E) :=
 
 theorem eq_of_indep_eq : ∀ {M₁ M₂ : indep E}, M₁.1 = M₂.1 → M₁ = M₂
   | ⟨I₁, p₁, q₁, r₁, s₁⟩ ⟨I₂, p₂, q₂, r₂, s₂⟩ h :=
-by simpa
+by simpa only []
 
 /-- A circuit of a matroid is a minimal dependent subset of the ground set -/
 def is_circuit (x : finset α) (m : indep E) : Prop :=
@@ -124,7 +123,7 @@ x ∉ m.indep ∧ ∀ y, y ⊂ x → y ∈ m.indep
 instance decidable_circuit (x : finset α) (m : indep E) : decidable (is_circuit x m) :=
 decidable_of_iff (x ∉ m.indep ∧ ∀ y ∈ (powerset x).erase x, y ∈ m.indep)
 begin
-  simp [is_circuit, (⊂)],
+  simp only [is_circuit, has_ssubset.ssubset, mem_powerset, and_imp, mem_erase],
   refine and_congr iff.rfl (forall_congr $ λ y, _),
   refine ⟨λ H h₁ h₂, H (mt _ h₂) h₁, λ H h₁ h₂, H h₂ $ mt _ h₁⟩,
   { rintro rfl, refl }, { exact subset.antisymm h₂ }
@@ -132,7 +131,8 @@ end
 
 instance decidable_circuit_subset (x : finset α) (m : indep E) :
   decidable (∃ (y : finset α) (H : y ⊆ x), is_circuit y m) :=
-decidable_of_iff (∃ (y : finset α) (H : y ∈ powerset x), is_circuit y m) $ by simp
+decidable_of_iff (∃ (y : finset α) (H : y ∈ powerset x), is_circuit y m) $
+  by simp only [exists_prop, mem_powerset]
 
 /- should I make this definition reducible? I don't know when to use attributes... -/
 def circuits_circ_of_indep (m : indep E) : finset (finset α) :=
@@ -141,7 +141,7 @@ def circuits_circ_of_indep (m : indep E) : finset (finset α) :=
 lemma C2_of_indep (m : indep E) (x y : finset α) (hx : x ∈ circuits_circ_of_indep m)
   (hy : y ∈ circuits_circ_of_indep m) (hxy : x ⊆ y) : x = y :=
 begin
-  simp [circuits_circ_of_indep, is_circuit] at *,
+  simp only [circuits_circ_of_indep, is_circuit, mem_filter] at *,
   have hnxy : ¬x ⊂ y := λ h, hx.2.1 $ hy.2.2 x h,
   rw ←lt_iff_ssubset at hnxy, rw [←le_iff_subset, le_iff_eq_or_lt] at hxy,
   exact or.elim hxy id (λ hxy2, false.elim $ hnxy hxy2)
@@ -153,10 +153,10 @@ theorem dep_iff_circuit_subset {x : finset α} (m : indep E) :
     mem_filter.mpr ⟨mem_powerset.mpr $ subset.refl x, hxd⟩)) $
   λ a ha, exists.elim ha $
     λ ha2 hamin, exists.intro a $ have hax : a ⊆ x := mem_powerset.mp (mem_filter.mp ha2).1,
-      exists.intro hax $ by unfold is_circuit;
+      exists.intro hax $ by { unfold is_circuit,
         exact ⟨(mem_filter.mp ha2).2, by { intros y hy, by_contra h,
           exact not_le_of_lt (card_lt_card hy) (hamin y $ mem_filter.mpr ⟨mem_powerset.mpr $
-            subset.trans (le_of_lt $ lt_iff_ssubset.mpr hy) hax, h⟩) }⟩) $
+            subset.trans (le_of_lt $ lt_iff_ssubset.mpr hy) hax, h⟩) }⟩ }) $
   λ H, exists.elim H $ λ a ha, exists.elim ha $
     by { intros hax hacirc hxi, unfold is_circuit at hacirc,
     exact hacirc.1 (m.indep_of_subset_indep hxi hax) }
@@ -168,14 +168,15 @@ lemma C3_of_indep (m : indep E) (x y : finset α) (e : α) (hx : x ∈ circuits_
 have hxmy : x \ y ≠ ∅ := mt subset_iff_sdiff_eq_empty.mpr $ mt (C2_of_indep m x y hx hy) hxny,
   exists.elim (exists_mem_of_ne_empty hxmy) $
     by { clear hxny hxmy,
-    intros a ha, simp [circuits_circ_of_indep] at ha hx hy he,
-    have hxai : erase x a ∈ m.indep := by unfold is_circuit at hx;
-      exact hx.2.2 (erase x a) (erase_ssubset ha.1),
+    intros a ha, simp only [circuits_circ_of_indep, mem_powerset, mem_filter, mem_sdiff, mem_inter]
+      at ha hx hy he,
+    have hxai : erase x a ∈ m.indep := by { unfold is_circuit at hx,
+      exact hx.2.2 (erase x a) (erase_ssubset ha.1) },
     let F := (powerset (x ∪ y)).filter (λ S, erase x a ⊆ S ∧ S ∈ m.indep),
     have hxaF : erase x a ∈ F := mem_filter.2 ⟨mem_powerset.mpr $ subset.trans (erase_subset a x) $
       @subset_union_left _ _ x y, ⟨subset.refl _, hxai⟩⟩, clear hxai,
     exact exists.elim (max_fun_of_ne_empty card $ ne_empty_of_mem hxaF)
-      (λ I hEI2, exists.elim hEI2 $ by clear hxaF hEI2;
+      (λ I hEI2, exists.elim hEI2 $ by { clear hxaF hEI2,
         exact λ hIF hI,
           have hIFindep : I ∈ m.indep := (mem_filter.mp hIF).2.2,
           have hIdep : _ → I ∉ m.indep := (dep_iff_circuit_subset m $ mem_powerset.1 $
@@ -187,11 +188,12 @@ have hxmy : x \ y ≠ ∅ := mt subset_iff_sdiff_eq_empty.mpr $ mt (C2_of_indep 
               have ∃ A ⊆ I, is_circuit A m := exists.intro x (exists.intro hxI hx.2),
               hIdep this hIFindep,
           have hEg : ∃ g ∈ y, g ∉ I :=
-            by { have hIdep2 := mt hIdep, simp at hIdep2,
-            have hyI0 := mt (hIdep2 hIFindep y), simp at hyI0,
+            by { have hIdep2 := mt hIdep, simp only [not_exists, exists_prop, not_and, not_not]
+              at hIdep2,
+            have hyI0 := mt (hIdep2 hIFindep y), simp only [not_not] at hyI0,
             have hYI : ¬y ⊆ I := hyI0 hy.2,
             have this := exists_mem_of_ne_empty (mt subset_iff_sdiff_eq_empty.mpr hYI),
-            simp at this, simpa },
+            simp only [mem_sdiff] at this, simpa only [exists_prop] },
           exists.elim hEg $ λ g hEg2, exists.elim hEg2 $ by { clear hEg hEg2 hIdep,
             intros hgy hgnI,
             have hga : g ≠ a := λ H, ha.2 (H ▸ hgy),
@@ -201,8 +203,8 @@ have hxmy : x \ y ≠ ∅ := mt subset_iff_sdiff_eq_empty.mpr $ mt (C2_of_indep 
             have haxuy : a ∈ x ∪ y := mem_union_left y ha.1,
             have hcardxye : card (erase (x ∪ y) a) = nat.pred (card (x ∪ y)) :=
               card_erase_of_mem haxuy,
-            have hpcard : nat.pred (card (x ∪ y)) > 0 := by rw ←hcardxye;
-              exact card_pos.mpr (ne_empty_of_mem $ mem_erase.mpr ⟨hga, mem_union_right x hgy⟩),
+            have hpcard : nat.pred (card (x ∪ y)) > 0 := by { rw ←hcardxye,
+              exact card_pos.mpr (ne_empty_of_mem $ mem_erase.mpr ⟨hga, mem_union_right x hgy⟩) },
             have hcard : card I < card (erase (x ∪ y) e) :=
               calc card I ≤ card (erase (erase (x ∪ y) a) g) : card_le_of_subset hIag
               ... = nat.pred (nat.pred (card (x ∪ y))) : by rw [card_erase_of_mem
@@ -211,12 +213,14 @@ have hxmy : x \ y ≠ ∅ := mt subset_iff_sdiff_eq_empty.mpr $ mt (C2_of_indep 
                 by { rw [card_erase_of_mem (mem_union_left y he.1),
                 ←nat.succ_pred_eq_of_pos hpcard], exact nat.lt_succ_self _ },
             clear hga hIag haxuy hcardxye hpcard he,
-            by_contra h, simp [circuits_circ_of_indep] at h,
+            by_contra h, simp only [circuits_circ_of_indep, mem_powerset, not_exists, and_imp,
+              mem_filter, not_and] at h,
             have hinE : erase (x ∪ y) e ⊆ E :=
               subset.trans (erase_subset e (x ∪ y)) (union_subset hx.1 hy.1),
             have : (∀ x_1 : finset α, x_1 ⊆ erase (x ∪ y) e → ¬is_circuit x_1 m) :=
               λ x1 hx1, (mt $ h x1 $ subset.trans hx1 hinE) $ not_not.mpr hx1,
-            have hindep := mt (dep_iff_circuit_subset m hinE).mp, simp at hindep,
+            have hindep := mt (dep_iff_circuit_subset m hinE).mp,
+              simp only [not_exists, exists_prop, not_and, not_not] at hindep,
             replace hindep : erase (x ∪ y) e ∈ m.indep := hindep this,
             have hfinal := m.indep_exch hIFindep hindep hcard,
             exact exists.elim hfinal (λ El ⟨hElxy, hElindep⟩,
@@ -226,7 +230,7 @@ have hxmy : x \ y ≠ ∅ := mt subset_iff_sdiff_eq_empty.mpr $ mt (C2_of_indep 
               have hcardEl : card I < card (insert El I) :=
                 by { rw card_insert_of_not_mem (mem_sdiff.mp hElxy).2,
                 exact lt_add_one (card I) },
-              not_lt.mpr (hI (insert El I) hElF) hcardEl) } ) }
+              not_lt.mpr (hI (insert El I) hElF) hcardEl) } }) }
 
 structure circuits (E : finset α) :=
 (circuits : finset (finset α))
@@ -245,14 +249,18 @@ instance circuits_repr [has_repr α] (E : finset α) : has_repr (circuits E) :=
 
 theorem eq_of_circ_eq : ∀ {C₁ C₂ : circuits E}, C₁.1 = C₂.1 → C₁ = C₂
   | ⟨c₁, p₁, q₁, r₁, s₁⟩ ⟨c₂, p₂, q₂, r₂, s₂⟩ h :=
-by simpa
+by simpa only []
 
 def circuits_of_indep (m : indep E) : circuits E :=
-⟨circuits_circ_of_indep m,
-filter_subset _,
-by simp [circuits_circ_of_indep, is_circuit]; exact λ h h1, h m.empty_mem_indep,
-C2_of_indep m,
-C3_of_indep m⟩
+{ circuits := circuits_circ_of_indep m,
+  circuits_subset_powerset_ground := filter_subset _,
+  empty_not_mem_circuits :=
+    begin
+      simp only [circuits_circ_of_indep, is_circuit, mem_filter, not_and],
+      exact λ h h1, (h1 m.empty_mem_indep).elim
+    end,
+  circuits_eq_of_subset := C2_of_indep m,
+  circuit_elim := C3_of_indep m }
 
 /- make reducible? -/
 def indep_indep_of_circuits (C : circuits E) : finset (finset α) :=
@@ -261,16 +269,20 @@ def indep_indep_of_circuits (C : circuits E) : finset (finset α) :=
 /-- first part of Theorem 1.1.4 -/
 lemma I2_of_circuits (C : circuits E) (x y : finset α) : x ∈ indep_indep_of_circuits C → y ⊆ x →
   y ∈ indep_indep_of_circuits C :=
-by unfold indep_indep_of_circuits at *; simp at *;
+begin
+  simp only [indep_indep_of_circuits, mem_powerset, and_imp, mem_filter],
   exact λ hxE hx hxy, ⟨subset.trans hxy hxE, λ c hc H, hx c hc $ subset.trans H hxy⟩
+end
 
 /-- second part of Theorem 1.1.4 -/
 lemma I3_of_circuits (C : circuits E) (x y : finset α) (hx : x ∈ indep_indep_of_circuits C)
   (hy : y ∈ indep_indep_of_circuits C) (hcardxy : card x < card y)
   : ∃ e, e ∈ y \ x ∧ insert e x ∈ indep_indep_of_circuits C :=
 begin
-  unfold indep_indep_of_circuits at *, simp at hx hy,
-  by_contra h, simp at h,
+  unfold indep_indep_of_circuits at ⊢,
+  simp only [indep_indep_of_circuits, mem_powerset, mem_filter] at hx hy,
+  by_contra h,
+  simp only [mem_powerset, not_exists, and_imp, mem_filter, not_and, mem_sdiff] at h,
   let F := (powerset $ x ∪ y).filter (λ S, (∀ c ∈ C.circuits, ¬c ⊆ S) ∧ card x < card S),
   have hyF : y ∈ F := mem_filter.mpr ⟨mem_powerset.mpr $ subset_union_right x y,
     ⟨hy.2, hcardxy⟩⟩,
@@ -280,60 +292,63 @@ begin
       have hzxuy : z ⊆ x ∪ y := mem_powerset.mp (mem_filter.mp hz).1,
       replace hz := (mem_filter.mp hz).2,
       exact exists.elim (exists_sdiff_of_card_lt hz.2)
-        (by { intros a ha, simp at ha,
+        (by { intros a ha, rw mem_sdiff at ha,
         have hxsdiffz : x \ z ≠ ∅ :=
           by { intro H,
           have Hxsubz : x ⊆ z := subset_iff_sdiff_eq_empty.mpr H,
           have hay : a ∈ y := or.elim (mem_union.mp $ mem_of_subset hzxuy ha.1)
             (λ Hax, false.elim $ ha.2 Hax) id,
           have haindep : insert a x ∈ indep_indep_of_circuits C := I2_of_circuits C z (insert a x)
-            (by simp [indep_indep_of_circuits];
-            exact ⟨subset.trans hzxuy $ union_subset hx.1 hy.1, hz.1⟩)
+            (by { simp only [indep_indep_of_circuits, mem_powerset, mem_filter],
+            exact ⟨subset.trans hzxuy $ union_subset hx.1 hy.1, hz.1⟩ })
             (insert_subset.mpr ⟨ha.1, Hxsubz⟩),
-          unfold indep_indep_of_circuits at haindep, simp at haindep,
+          simp only [indep_indep_of_circuits, mem_powerset, mem_filter] at haindep,
           exact h a hay ha.2 haindep.1 haindep.2 },
         exact exists.elim (exists_mem_of_ne_empty hxsdiffz)
           (by { clear h ha hxsdiffz,
-          intros e he, simp at he,
+          intros e he, rw mem_sdiff at he,
           let T : α → finset α := λ f, erase (insert e z) f,
           have hTf1 : ∀ f, f ∈ z \ x → T f ⊆ x ∪ y :=
-            by { intros f hf, simp at hf,
+            by { intros f hf, rw [mem_sdiff] at hf,
             rw [subset_iff],
-            intros gg hgg, simp at hgg,
-            simp,
+            intros gg hgg, simp only [mem_insert, mem_erase, ne.def] at hgg,
+            simp only [mem_union],
             exact or.elim hgg.2 (λ gge, or.inl $ gge.symm ▸ he.1)
               (λ ggz, mem_union.mp $ mem_of_subset hzxuy ggz) },
           have hTf2 : ∀ f, f ∈ z \ x → card (x \ T f) < card (x \ z) :=
-            by { intros f hf, simp at hf,
+            by { intros f hf, rw mem_sdiff at hf,
             suffices H : x \ T f ⊂ x \ z, exact card_lt_card H,
-            by simp [ssubset_iff]; exact exists.intro e
-              ⟨λ h_, ⟨λ hef, hf.2 $ hef ▸ he.1, or.inl rfl⟩,
-              by { rw [subset_iff],
-                intros gg hgg, simp at hgg,
-                have ggnef : gg ≠ f := λ ggef, or.elim hgg
-                  (λ gge, (gge.symm ▸ he.2) $ ggef.substr hf.1) (λ H, (ggef.substr hf.2) H.1),
-                have he0 := mem_sdiff.mpr he,
-                exact or.elim hgg (λ gge, gge.symm ▸ he0)
-                (λ H, mem_sdiff.mpr ⟨H.1, λ ggz, (H.2 ggnef) $ or.inr ggz⟩) }⟩ },
+            by { simp only [ssubset_iff, exists_prop, mem_insert, not_forall_not, not_and,
+                            mem_sdiff, mem_erase],
+              exact exists.intro e
+                ⟨λ h_, ⟨λ hef, hf.2 $ hef ▸ he.1, or.inl rfl⟩,
+                by { rw [subset_iff],
+                  intros gg hgg,
+                  simp only [mem_insert, not_and, mem_sdiff, mem_erase, ne.def] at hgg,
+                  have ggnef : gg ≠ f := λ ggef, or.elim hgg
+                    (λ gge, (gge.symm ▸ he.2) $ ggef.substr hf.1) (λ H, (ggef.substr hf.2) H.1),
+                  have he0 := mem_sdiff.mpr he,
+                  exact or.elim hgg (λ gge, gge.symm ▸ he0)
+                  (λ H, mem_sdiff.mpr ⟨H.1, λ ggz, (H.2 ggnef) $ or.inr ggz⟩) }⟩ } },
           have hTfindep : ∀ f, f ∈ z \ x → T f ∉ indep_indep_of_circuits C :=
             by { intros f hf,
-            unfold indep_indep_of_circuits, simp,
+            simp only [indep_indep_of_circuits, mem_powerset, mem_filter, not_and],
             intros hTfE H,
             have HTf1 : T f ⊆ x ∪ y := hTf1 f hf,
             have HTf2 : card (x \ T f) < card (x \ z) := hTf2 f hf,
-            simp at hf,
+            rw mem_sdiff at hf,
             have HTfcard : card z = card (T f) :=
-              by { simp [card_erase_of_mem (mem_insert.mpr $ or.inr hf.1),
-              card_insert_of_not_mem he.2] },
+              by { simp only [card_erase_of_mem (mem_insert.mpr $ or.inr hf.1),
+              card_insert_of_not_mem he.2, mem_insert, card_insert_of_not_mem, nat.pred_succ] },
             replace HTfcard : card x < card (T f) := HTfcard ▸ hz.2,
             have : T f ∈ F := mem_filter.mpr ⟨mem_powerset.mpr HTf1, ⟨H, HTfcard⟩⟩,
             exact not_lt.mpr (hminz (T f) this) HTf2 },
           have hTfC : ∀ f, f ∈ z \ x → ∃ c ∈ C.circuits, c ⊆ T f :=
             by { intros f hf,
             have : T f ∉ indep_indep_of_circuits C := hTfindep f hf,
-              simp [indep_indep_of_circuits] at this,
+              simp only [indep_indep_of_circuits, mem_powerset, mem_filter, not_and] at this,
             have hfc := this (subset.trans (hTf1 f hf) $ union_subset hx.1 hy.1),
-            by_contra H, simp at H, contradiction },
+            by_contra H, simp only [not_exists, exists_prop, not_and] at H, contradiction },
           exact exists.elim (exists_sdiff_of_card_lt hz.2) (λ g hg, exists.elim (hTfC g hg) $
               λ Cg hCg, exists.elim hCg $
                 by { clear hCg hTf1 hTf2 hTfindep hg,
@@ -347,16 +362,19 @@ begin
                     subset.trans H1 H2,
                     show erase (insert e (x ∩ z)) g ⊆ x, by
                       { rw [subset_iff],
-                      intros gg hgg, simp at hgg,
+                      intros gg hgg,
+                      simp only [mem_insert, mem_erase, mem_inter] at hgg,
                       exact or.elim hgg.2 (λ gge, gge.symm ▸ he.1) (λ ggxggz, ggxggz.1) },
                     show Cg ⊆ erase (insert e (x ∩ z)) g, by
                       { rw [subset_iff],
                       intros gg hgg,
-                      replace HCg2 : gg ∈ T g := HCg2 hgg, simp at HCg2,
-                      simp, split,
+                      replace HCg2 : gg ∈ T g := HCg2 hgg,
+                      simp only [mem_insert, mem_erase, mem_inter] at HCg2 ⊢,
+                      split,
                         { exact HCg2.1 },
                         { rw eq_empty_iff_forall_not_mem at H,
-                        replace H : gg ∉ Cg ∩ (z \ x) := H gg, simp at H,
+                        replace H : gg ∉ Cg ∩ (z \ x) := H gg,
+                        simp only [not_and, mem_sdiff, not_not, mem_inter] at H,
                       exact or.elim HCg2.2 (λ gge, or.inl gge) (λ ggz, or.inr ⟨H hgg ggz, ggz⟩) } },
                 clear HCg2,
                 exact exists.elim (exists_mem_of_ne_empty HCgzx)
@@ -369,7 +387,7 @@ begin
                       have hCh0sub : Ch0 ⊆ insert e z :=
                         subset.trans hCh0T (erase_subset h0 $ insert e z),
                       have heCgCh0 : e ∈ Cg ∩ Ch0 :=
-                        by { simp, split,
+                        by { rw mem_inter, split,
                           { by_contra heCg, have hCgz : Cg ⊆ z :=
                               (erase_eq_of_not_mem heCg) ▸ (subset_insert_iff.mp hCgsub),
                             exact hz.1 Cg HCg1 hCgz },
@@ -382,7 +400,8 @@ begin
                             by { rw [subset_iff],
                             intros t ht,
                             rw [subset_iff] at hCCCguCh0,
-                            have htCguCh0 := hCCCguCh0 ht, simp at htCguCh0,
+                            have htCguCh0 := hCCCguCh0 ht,
+                              simp only [mem_union, mem_erase] at htCguCh0,
                             rw [subset_iff] at hCgsub hCh0sub,
                             have orCg : t ∈ Cg → t ∈ z :=
                               λ htCg, or.elim (mem_insert.mp $ hCgsub htCg)
@@ -396,7 +415,7 @@ end
 
 def indep_of_circuits (C : circuits E) : indep E :=
 ⟨indep_indep_of_circuits C,
-by simp [indep_indep_of_circuits],
+by simp only [indep_indep_of_circuits, filter_subset],
 mem_filter.mpr
   ⟨empty_mem_powerset E, λ c hc H, C.empty_not_mem_circuits $ (subset_empty.mp H) ▸ hc⟩,
 I2_of_circuits C,
@@ -408,30 +427,34 @@ instance indep_circ : has_coe (indep E) (circuits E) := ⟨circuits_of_indep⟩
 /-- third part of Theorem 1.1.4 -/
 theorem circ_indep_circ : ∀ C : circuits E, C = circuits_of_indep (indep_of_circuits C)
   | ⟨c₁, p₁, q₁, r₁, s₁⟩ :=
-by simp [indep_of_circuits, circuits_of_indep, indep_indep_of_circuits, circuits_circ_of_indep, is_circuit, ext];
+by { simp only [indep_of_circuits, circuits_of_indep, indep_indep_of_circuits,
+  circuits_circ_of_indep, is_circuit, ext, mem_filter, mem_powerset, and_imp, not_and],
 exact λ c, iff.intro
   (λ hc : c ∈ c₁, have ce : c ⊆ E := mem_powerset.mp (mem_of_subset p₁ hc),
   ⟨ce, ⟨λ _ H, (H c hc) $ subset.refl c, λ f hf,
     ⟨subset.trans (le_of_lt $ lt_iff_ssubset.mpr hf) ce,
     λ g hg H, have Hc : g < c := lt_of_le_of_lt (le_iff_subset.mpr H) $ lt_iff_ssubset.mpr hf,
       have r : g = c := r₁ hg hc $ le_of_lt Hc, (not_le_of_lt Hc) $ le_of_eq r.symm⟩⟩⟩) $
-  λ hc, have ∃ c_1 ∈ c₁, c_1 ⊆ c := by { have := not_forall.mp (hc.2.1 hc.1), simpa },
+  λ hc, have ∃ c_1 ∈ c₁, c_1 ⊆ c := by { have := not_forall.mp (hc.2.1 hc.1),
+    simpa only [exists_prop, not_forall_not] },
   exists.elim this $ λ c' H, exists.elim H $ by { intros hc' hcc',
     by_cases h : c = c', { exact h.symm ▸ hc' },
       { have hc'lt : c' ⊂ c := lt_of_le_of_ne (le_iff_subset.mpr hcc') (ne.symm h),
         have : c' ∉ c₁ := mt ((hc.2.2 c' hc'lt).2 c') (not_not.mpr $ subset.refl c'),
-        exact false.elim (this hc') } }
+        exact false.elim (this hc') } } }
 
 theorem indep_circ_indep (M : indep E) : M = indep_of_circuits (circuits_of_indep M) :=
 suffices M.indep = (indep_of_circuits $ circuits_of_indep M).indep, from eq_of_indep_eq this,
 begin
-  simp [circuits_of_indep, indep_of_circuits, circuits_circ_of_indep, indep_indep_of_circuits, ext],
+  simp only [circuits_of_indep, indep_of_circuits, circuits_circ_of_indep, indep_indep_of_circuits,
+    ext, mem_powerset, and_imp, mem_filter],
   intro I,
   have hI : I ∈ M.indep → I ⊆ E := λ H, mem_powerset.mp $
     mem_of_subset (M.indep_subset_powerset_ground) H,
   rw [←and_iff_right_of_imp hI, and_congr_right],
   intro hIE, have := not_iff_not_of_iff (dep_iff_circuit_subset M hIE),
-  simp at this, rw [this, forall_congr],
+  simp only [not_exists, exists_prop, not_and, not_not] at this,
+  rw [this, forall_congr],
   exact λ a, ⟨λ h h₁ h₂ h₃, (h h₃) h₂, λ h h₁ h₂, h (subset.trans h₁ hIE) h₂ h₁⟩
 end
 
@@ -440,7 +463,7 @@ theorem existsu_circuit_of_dep_of_insert_indep {I : finset α} {e : α} {m : ind
   (hI : I ∈ m.indep) (he : e ∈ E) (hIe : insert e I ∉ m.indep) :
   ∃ c, c ∈ circuits_circ_of_indep m ∧ c ⊆ insert e I ∧ e ∈ c ∧
   ∀ c' ∈ circuits_circ_of_indep m, c' ⊆ insert e I ∧ e ∈ c → c' = c :=
-by simp [circuits_circ_of_indep];
+by { simp only [circuits_circ_of_indep, mem_powerset, and_imp, mem_filter],
 exact have hIE : I ⊆ E, from mem_powerset.mp (mem_of_subset m.indep_subset_powerset_ground hI),
 have hIeE : insert e I ⊆ E, from insert_subset.mpr ⟨he, hIE⟩,
 have hc : _, from (dep_iff_circuit_subset m hIeE).mp hIe,
@@ -458,15 +481,18 @@ exists.elim hc $ λ c hEc, exists.elim hEc $ λ hceI hccirc,
   have hec : e ∈ c := hecirc c hceI hccirc,
   exists.intro c $ by { exact ⟨⟨hcE, hccirc⟩, ⟨hceI,⟨hec, by { intros c' hc'E hc'circ hc'eI _,
     have hec' : e ∈ c' := hecirc c' hc'eI hc'circ,
-    have hcuc'eI : erase (c ∪ c') e ⊆ I := by simp [subset_iff] at hceI hc'eI ⊢;
+    have hcuc'eI : erase (c ∪ c') e ⊆ I := by {
+      simp only [subset_iff, and_imp, mem_union, mem_insert, mem_erase, ne.def] at hceI hc'eI ⊢,
       exact λ a hane ha, or.elim ha (λ H, or.elim (hceI H) (λ H, false.elim $ hane H) id)
-        (λ H, or.elim (hc'eI H) (λ H, false.elim $ hane H) id),
+        (λ H, or.elim (hc'eI H) (λ H, false.elim $ hane H) id) },
     have : erase (c ∪ c') e ∈ m.indep := m.indep_of_subset_indep hI hcuc'eI,
     by_contra h,
-    have C3 := C3_of_indep m c c' e, simp [circuits_circ_of_indep] at C3,
+    have C3 := C3_of_indep m c c' e,
+      simp only [circuits_circ_of_indep, mem_powerset, and_imp,
+        filter_congr_decidable, mem_filter, mem_inter] at C3,
     exact exists.elim (C3 hcE hccirc hc'E hc'circ (ne.symm h) hec hec')
       (λ c₀ hc₀, (dep_iff_circuit_subset m hIE).mpr (exists.intro c₀ $ exists.intro
-        (subset.trans hc₀.2 hcuc'eI) hc₀.1.2) hI) }⟩⟩⟩ }
+        (subset.trans hc₀.2 hcuc'eI) hc₀.1.2) hI) }⟩⟩⟩ } }
 
 section encodable
 variable [encodable α]
@@ -492,7 +518,8 @@ def is_basis (x : finset α) (m : indep E) : Prop :=
 x ∈ m.indep ∧ (∀ y ⊆ E, x ⊂ y → y ∉ m.indep)
 
 instance decidable_basis (x : finset α) (m : indep E) : decidable (is_basis x m) :=
-decidable_of_iff (x ∈ m.indep ∧ (∀ y ∈ powerset E, x ⊂ y → y ∉ m.indep)) $ by simp [is_basis]
+decidable_of_iff (x ∈ m.indep ∧ (∀ y ∈ powerset E, x ⊂ y → y ∉ m.indep)) $
+  by simp only [is_basis, iff_self, finset.mem_powerset]
 
 /-- Lemma 1.2.1 -/
 theorem bases_of_indep_card_eq {x y : finset α} {m : indep E} : is_basis x m → is_basis y m →
@@ -502,7 +529,7 @@ begin
   by_contra heq,
   wlog h : card x < card y using [x y, y x],
   exact lt_or_gt_of_ne heq,
-  unfold is_basis at *,
+  unfold is_basis at hx hy,
   exact exists.elim (m.indep_exch hx.1 hy.1 h) (λ e ⟨he1, he2⟩,
     have hins : insert e x ⊆ E := mem_powerset.mp
       (mem_of_subset (m.indep_subset_powerset_ground) he2),
@@ -515,7 +542,7 @@ theorem exists_basis_containing_indep {I : finset α} {m : indep E} (h : I ∈ m
 let F := (m.indep).filter (λ a, I ⊆ a) in
 have FI : I ∈ F := mem_filter.mpr ⟨h, subset.refl I⟩,
 exists.elim (max_fun_of_ne_empty card $ ne_empty_of_mem FI) $
-  λ B HB, exists.elim HB $ by { clear HB, intros HBF Hg, simp at HBF,
+  λ B HB, exists.elim HB $ by { clear HB, intros HBF Hg, rw mem_filter at HBF,
     have hBB : is_basis B m := ⟨HBF.1, λ y hy hBy hyI,
       have hxsy : I ⊆ y := le_of_lt $ lt_of_le_of_lt (le_iff_subset.mpr HBF.2) $
         lt_iff_ssubset.mpr hBy,
@@ -544,7 +571,7 @@ theorem dep_of_card_gt_card_basis {x B : finset α} {m : indep E} (hB : is_basis
 
 theorem card_of_indep_le_card_basis {x B : finset α} {m : indep E} (hx : x ∈ m.indep)
   (hB : is_basis B m) : card x ≤ card B :=
-by by_contra h; exact dep_of_card_gt_card_basis hB (lt_of_not_ge h) hx
+by { by_contra h, exact dep_of_card_gt_card_basis hB (lt_of_not_ge h) hx }
 
 structure bases (E : finset α) :=
 (bases : finset (finset α))
@@ -561,23 +588,25 @@ instance bases_repr [has_repr α] (E : finset α) : has_repr (bases E) :=
 
 theorem eq_of_base_eq : ∀ {B₁ B₂ : bases E}, B₁.1 = B₂.1 → B₁ = B₂
   | ⟨b₁, p₁, q₁, r₁⟩ ⟨b₂, p₂, q₂, r₂⟩ h :=
-by simpa
+by simpa only []
 
 def bases_bases_of_indep (m : indep E) : finset (finset α) :=
 (powerset E).filter (λ S, is_basis S m)
 
 lemma B1_of_indep (m : indep E) : bases_bases_of_indep m ≠ ∅ :=
-by simp [is_basis, ext, bases_bases_of_indep];
-exact λ h, exists.elim (max_fun_of_ne_empty card $ ne_empty_of_mem m.empty_mem_indep)
+by { simp only [is_basis, bases_bases_of_indep, ext, ne.def, mem_filter, mem_powerset,
+    not_mem_empty, not_and, iff_false],
+  exact λ h, exists.elim (max_fun_of_ne_empty card $ ne_empty_of_mem m.empty_mem_indep)
   (λ a ha, exists.elim ha $ λ ha1 hg, (h a (mem_powerset.mp $
     mem_of_subset m.indep_subset_powerset_ground ha1)
-  ha1) $ λ F _ Fcontainsa Findep, not_le_of_lt (card_lt_card Fcontainsa) $ hg F Findep)
+  ha1) $ λ F _ Fcontainsa Findep, not_le_of_lt (card_lt_card Fcontainsa) $ hg F Findep) }
 
 /- Lemma 1.2.2 -/
 lemma B2_of_indep (m : indep E) : ∀ (x y : finset α) (e : α), x ∈ bases_bases_of_indep m →
   y ∈ bases_bases_of_indep m → e ∈ x \ y →
   ∃ a, a ∈ y \ x ∧ insert a (erase x e) ∈ bases_bases_of_indep m :=
-by simp [is_basis, bases_bases_of_indep];
+by { simp only [is_basis, bases_bases_of_indep, filter_and, mem_filter, mem_sdiff,
+  mem_powerset, and_imp],
 exact λ x y e hxE hxI hx hyE hyI hy hex hey,
   have hxr : erase x e ∈ m.indep := m.indep_of_subset_indep hxI $ erase_subset e x,
   have hxB : is_basis x m := ⟨hxI, hx⟩, have hyB : is_basis y m := ⟨hyI, hy⟩,
@@ -588,7 +617,7 @@ exact λ x y e hxE hxI hx hyE hyI hy hex hey,
     by { clear hxr hyI hcard hyB, intros a ha,
       have ha1 := mem_sdiff.mp ha.1,
       have hae : a ≠ e := λ hae, hey $ hae ▸ ha1.1,
-      have hax : a ∉ x := by simp at ha1; exact ha1.2 hae,
+      have hax : a ∉ x := by { simp only [not_and, mem_erase, ne.def] at ha1, exact ha1.2 hae },
       have hcx : card x > 0 := card_pos.mpr (ne_empty_of_mem hex),
       have hayycard : card (insert a $ erase x e) = card x := calc
         card (insert a $ erase x e) = nat.pred (card x) + 1 : by rw [card_insert_of_not_mem ha1.2,
@@ -596,7 +625,7 @@ exact λ x y e hxE hxI hx hyE hyI hy hex hey,
         ... = card x : nat.succ_pred_eq_of_pos hcx,
       exact exists.intro a ⟨⟨ha1.1, hax⟩, mem_powerset.mp $
         mem_of_subset m.indep_subset_powerset_ground ha.2, ha.2,
-        λ _ _ hayy, dep_of_card_gt_card_basis hxB $ hayycard ▸ (card_lt_card hayy)⟩ }
+        λ _ _ hayy, dep_of_card_gt_card_basis hxB $ hayycard ▸ (card_lt_card hayy)⟩ } }
 
 def bases_of_indep (m : indep E) : bases E :=
 ⟨bases_bases_of_indep m,
@@ -621,26 +650,26 @@ begin
       have hab : a.1 ∈ b.bases ∧ a.2 ∈ b.bases := mem_product.mp haF.1,
       exact exists.elim (exists_sdiff_of_card_lt haF.2)
         (λ e he, exists.elim (b.basis_exch hab.2 hab.1 he) $ λ aa ⟨haa1, haa2⟩,
-          by { simp at haa1,
+          by { rw mem_sdiff at haa1,
           let a2 : finset α := insert aa (erase a.2 e),
           have haani : aa ∉ erase a.2 e := λ h, haa1.2 (mem_erase.mp h).2,
           have hea2 : e ∈ a.2 := (mem_sdiff.mp he).1,
           have hpos : 0 < card a.2 := card_pos.mpr (ne_empty_of_mem hea2),
-          have hcarda2 : card a.1 < card a2 := by rw [card_insert_of_not_mem haani,
-            card_erase_of_mem hea2, ←nat.succ_eq_add_one, nat.succ_pred_eq_of_pos hpos];
-            exact haF.2, clear haani hpos,
+          have hcarda2 : card a.1 < card a2 := by { rw [card_insert_of_not_mem haani,
+            card_erase_of_mem hea2, ←nat.succ_eq_add_one, nat.succ_pred_eq_of_pos hpos],
+            exact haF.2 }, clear haani hpos,
           have : e ∉ a2 := λ hh, or.elim (mem_insert.mp hh)
             (λ h4, haa1.2 $ h4 ▸ hea2) $ λ h5, (mem_erase.mp h5).1 rfl,
           have hcard : card (a2 \ a.1) < card (a.2 \ a.1) :=
             suffices a2 \ a.1 ⊂ a.2 \ a.1, from card_lt_card this,
-            by rw ssubset_iff;
+            by { rw ssubset_iff,
             exact exists.intro e ⟨λ h0, this (mem_sdiff.mp h0).1,
               by { rw subset_iff,
               intros A hA, rw mem_insert at hA,
               exact or.elim hA (λ hA1, hA1.symm ▸ he)
                 (by { intro hA2, rw [mem_sdiff, mem_insert] at hA2,
                 exact mem_sdiff.mpr ⟨or.elim hA2.1 (λ h6, false.elim $ hA2.2 $ h6.symm ▸ haa1.1) $
-                  λ h7, (mem_erase.mp h7).2, hA2.2⟩ }) }⟩,
+                  λ h7, (mem_erase.mp h7).2, hA2.2⟩ }) }⟩ },
           have ha2F : (a.1, a2) ∈ F := mem_filter.mpr ⟨mem_product.mpr ⟨hab.1, haa2⟩, hcarda2⟩,
           exact not_le_of_lt hcard (Ha (a.1, a2) ha2F) }) })
 end
@@ -655,73 +684,80 @@ filter_subset _,
 mem_filter.mpr ⟨empty_mem_powerset E, exists.elim (exists_mem_of_ne_empty b.bases_not_empty) $
     λ a ha, exists.intro a $ exists.intro ha $ empty_subset a⟩,
 begin
-  intros x y hx hxy, simp [indep_indep_of_bases] at *,
+  intros x y hx hxy, simp only [indep_indep_of_bases, mem_powerset, filter_congr_decidable,
+    exists_prop, mem_filter] at hx ⊢,
   exact ⟨subset.trans hxy hx.1,
     exists.elim hx.2 $ λ a ha, exists.intro a ⟨ha.1, subset.trans hxy ha.2⟩⟩
 end,
 begin
   intros x y hx hy hcard, unfold indep_indep_of_bases at *,
   let F := (b.bases).filter (λ S, S ⊆ y),
-  by_contra h, simp at *,
+  by_contra h, simp only [mem_powerset, not_exists, and_imp, filter_congr_decidable,
+    exists_prop, mem_filter, not_and, mem_sdiff] at hx hy h,
   exact exists.elim hx.2 (λ b1 hb1, exists.elim hy.2 $ λ b2 hb2, exists.elim
     (min_fun_of_ne_empty (λ f, card (f \ (y ∪ b1))) $ ne_empty_of_mem $ mem_filter.mpr hb2) $
     λ B2 hEB2, exists.elim hEB2 $ by { clear hb2 b2 hEB2,
       intros hB2filt hB2min, replace hB2filt : B2 ∈ b.bases ∧ y ⊆ B2 := mem_filter.mp hB2filt,
-      have hysdiff : y \ b1 = y \ x := by simp [ext];
+      have hysdiff : y \ b1 = y \ x := by { simp only [ext, mem_sdiff],
         exact λ gg, ⟨λ hgg, ⟨hgg.1, λ hggnx, hgg.2 $ mem_of_subset hb1.2 hggnx⟩,
           λ hgg, ⟨hgg.1, λ ggb1, h gg hgg.1 hgg.2 (insert_subset.mpr
-          ⟨mem_of_subset hy.1 hgg.1, hx.1⟩) b1 hb1.1 $ insert_subset.mpr ⟨ggb1, hb1.2⟩⟩⟩,
-      have hB2yub1: B2 \ (y ∪ b1) = ∅ := by by_contra H;
+          ⟨mem_of_subset hy.1 hgg.1, hx.1⟩) b1 hb1.1 $ insert_subset.mpr ⟨ggb1, hb1.2⟩⟩⟩ },
+      have hB2yub1: B2 \ (y ∪ b1) = ∅ := by { by_contra H,
         exact exists.elim (exists_mem_of_ne_empty H) (by { clear H,
-          intros X hX, simp [not_or_distrib] at hX,
-          have hXB2b1 : X ∈ B2 \ b1 := by simp; exact ⟨hX.1, hX.2.2⟩,
+          intros X hX, simp only [not_or_distrib, mem_union, mem_sdiff] at hX,
+          have hXB2b1 : X ∈ B2 \ b1 := by { rw mem_sdiff, exact ⟨hX.1, hX.2.2⟩ },
           exact exists.elim (b.basis_exch hB2filt.1 hb1.1 hXB2b1)
-            (λ Y ⟨hYb1B2, hYbases⟩, by { simp at hYb1B2 hXB2b1,
+            (λ Y ⟨hYb1B2, hYbases⟩, by { rw mem_sdiff at hYb1B2 hXB2b1,
               have hssubY : insert Y (erase B2 X) \ (y ∪ b1) ⊂  B2 \ (y ∪ b1) :=
-                by rw [ssubset_iff];
-                exact exists.intro X (by simp [subset_iff, not_or_distrib];
+                by { rw [ssubset_iff],
+                exact exists.intro X (by {
+                  simp only [subset_iff, not_or_distrib, mem_union, mem_insert, not_and, mem_sdiff,
+                    not_not, mem_erase, not_true, or_false, ne.def, false_and, or_false,
+                    eq_self_iff_true],
                   exact ⟨λ hXY, false.elim $ hYb1B2.2 (hXY ▸ hXB2b1.1),
                   λ gg hgg, or.elim hgg (λ ggx, ggx.symm ▸ hX) $ λ ggor2, or.elim ggor2.1
                     (λ ggY, false.elim $ (ggY ▸ ggor2.2.2) hYb1B2.1) $
-                      λ ggXB2, ⟨ggXB2.2, ggor2.2⟩⟩),
+                      λ ggXB2, ⟨ggXB2.2, ggor2.2⟩⟩ }) },
               replace hssubY := card_lt_card hssubY,
-              have hysubY : y ⊆ insert Y (erase B2 X) := by simp [subset_iff];
-                exact λ gg hgg, or.inr ⟨λ ggx, hX.2.1 $ ggx ▸ hgg, mem_of_subset hB2filt.2 hgg⟩,
+              have hysubY : y ⊆ insert Y (erase B2 X) := by {
+                simp only [subset_iff, mem_insert, mem_erase, ne.def],
+                exact λ gg hgg, or.inr ⟨λ ggx, hX.2.1 $ ggx ▸ hgg, mem_of_subset hB2filt.2 hgg⟩ },
               exact not_lt_of_le (hB2min (insert Y $ erase B2 X) $ mem_filter.mpr
-                  ⟨hYbases, hysubY⟩) hssubY }) }), clear hB2min,
-      rw [←subset_iff_sdiff_eq_empty, subset_iff] at hB2yub1, simp at hB2yub1,
-      have hB2b1y : B2 \ b1 = y \ b1 := by simp [ext];
+                  ⟨hYbases, hysubY⟩) hssubY }) }) }, clear hB2min,
+      rw [←subset_iff_sdiff_eq_empty, subset_iff] at hB2yub1, simp only [mem_union] at hB2yub1,
+      have hB2b1y : B2 \ b1 = y \ b1 := by { simp only [ext, mem_sdiff],
         exact λ gg, ⟨λ hgg, ⟨or.elim (hB2yub1 hgg.1) id $ λ hb1, false.elim $ hgg.2 hb1, hgg.2⟩,
-            λ hgg, ⟨mem_of_subset hB2filt.2 hgg.1, hgg.2⟩⟩,
+            λ hgg, ⟨mem_of_subset hB2filt.2 hgg.1, hgg.2⟩⟩ },
       rw [hysdiff] at hB2b1y, clear hysdiff,
-      have hb1xuB2 : b1 \ (x ∪ B2) = ∅ := by by_contra H;
+      have hb1xuB2 : b1 \ (x ∪ B2) = ∅ := by { by_contra H,
         exact exists.elim (exists_mem_of_ne_empty H)
-          (by { intros X hX, simp [not_or_distrib] at hX,
+          (by { intros X hX, simp only [not_or_distrib, mem_union, mem_sdiff] at hX,
           exact exists.elim (b.basis_exch hb1.1 hB2filt.1 $ mem_sdiff.mpr ⟨hX.1, hX.2.2⟩)
-            (by { intros Y hY, simp at hY,
+            (by { intros Y hY, rw mem_sdiff at hY,
             have hYyx : Y ∈ y ∧ Y ∉ x := mem_sdiff.mp (hB2b1y ▸ (mem_sdiff.mpr hY.1)),
-            have hxYsub : insert Y x ⊆ insert Y (erase b1 X) := by simp [subset_iff];
+            have hxYsub : insert Y x ⊆ insert Y (erase b1 X) := by {
+              simp only [subset_iff, mem_insert, mem_erase, ne.def],
               exact λ gg hgg, or.elim hgg (λ ggY, or.inl ggY) $ λ ggx, or.inr ⟨λ ggX, hX.2.1 $
-                ggX ▸ ggx, mem_of_subset hb1.2 ggx⟩,
+                ggX ▸ ggx, mem_of_subset hb1.2 ggx⟩ },
             have : insert Y x ⊆ E := insert_subset.mpr ⟨mem_of_subset hy.1 hYyx.1, hx.1⟩,
-            exact h Y hYyx.1 hYyx.2 this (insert Y $ erase b1 X) hY.2 hxYsub }) }),
+            exact h Y hYyx.1 hYyx.2 this (insert Y $ erase b1 X) hY.2 hxYsub }) }) },
       clear h hx hy,
-      rw [←subset_iff_sdiff_eq_empty, subset_iff] at hb1xuB2, simp at hb1xuB2,
-      have hb1B2 : b1 \ B2 = x \ B2 := by simp [ext];
+      rw [←subset_iff_sdiff_eq_empty, subset_iff] at hb1xuB2, simp only [mem_union] at hb1xuB2,
+      have hb1B2 : b1 \ B2 = x \ B2 := by { simp only [ext, mem_sdiff],
         exact λ gg, ⟨λ hgg, ⟨or.elim (hb1xuB2 hgg.1) id $ λ ggB2, false.elim $ hgg.2 ggB2, hgg.2⟩,
-            λ hgg, ⟨mem_of_subset hb1.2 hgg.1, hgg.2⟩⟩, clear hb1xuB2,
+            λ hgg, ⟨mem_of_subset hb1.2 hgg.1, hgg.2⟩⟩ }, clear hb1xuB2,
       replace hb1B2 : b1 \ B2 ⊆ x \ y := hb1B2.symm ▸ (sdiff_subset_sdiff (subset.refl x)
           hB2filt.2),
       have hcardeq : card b1 = card B2 := bases_card_eq hb1.1 hB2filt.1,
       have hcardb1B2 : card (b1 \ B2) = card (B2 \ b1) := calc
-        card (b1 \ B2) = card b1 - card (b1 ∩ B2) : card_sdiff b1 B2
+        card (b1 \ B2) = card b1 - card (b1 ∩ B2) : card_sdiff_eq b1 B2
         ... = card B2 - card (B2 ∩ b1) : by rw [hcardeq, inter_comm]
-        ... = card (B2 \ b1) : by rw ←card_sdiff B2 b1,
+        ... = card (B2 \ b1) : by rw ←card_sdiff_eq B2 b1,
       have hcardcontra0 : card (y \ x) ≤ card (x \ y) := calc
         card (y \ x) = card (B2 \ b1) : by rw hB2b1y
         ... = card (b1 \ B2) : by rw hcardb1B2
         ... ≤ card (x \ y) : card_le_of_subset hb1B2,
-      rw [card_sdiff y x, card_sdiff x y, inter_comm] at hcardcontra0,
+      rw [card_sdiff_eq y x, card_sdiff_eq x y, inter_comm] at hcardcontra0,
       have hcardcontra : card y ≤ card x := nat.le_of_le_of_sub_le_sub_right
           (card_le_of_subset $ @inter_subset_left _ _ x y) hcardcontra0,
       exact not_lt_of_le hcardcontra hcard })
@@ -733,7 +769,8 @@ instance indep_base : has_coe (indep E) (bases E) := ⟨bases_of_indep⟩
 /-- second part of Theorem 1.2.3 -/
 theorem base_indep_base (B : bases E) : B = bases_of_indep (indep_of_bases B) :=
 suffices B.bases = (bases_of_indep $ indep_of_bases B).bases, from eq_of_base_eq this,
-by simp [indep_of_bases, bases_of_indep, indep_indep_of_bases, is_basis, ext, bases_bases_of_indep];
+by { simp only [indep_of_bases, bases_of_indep, indep_indep_of_bases, is_basis,
+  ext, bases_bases_of_indep, mem_filter, mem_powerset, not_and, not_exists, exists_prop],
 exact λ b, iff.intro
   (λ hb, have hB : b ⊆ E := mem_powerset.mp (mem_of_subset B.bases_subset_powerset_ground hb),
     ⟨hB, ⟨⟨hB, exists.intro b ⟨hb, subset.refl b⟩⟩, λ b' _ hbb' _ _ hx H,
@@ -742,22 +779,23 @@ exact λ b, iff.intro
     B.bases_subset_powerset_ground ha.1, by { by_cases h : a = b,
       { exact h ▸ ha.1 },
       { have hba : b ⊂ a := lt_iff_ssubset.mp (lt_of_le_of_ne (le_iff_subset.mpr ha.2) $ ne.symm h),
-        exact false.elim (hb.2.2 a this hba this a ha.1 $ subset.refl a) } }
+        exact false.elim (hb.2.2 a this hba this a ha.1 $ subset.refl a) } } }
 
 theorem indep_base_indep (M : indep E) : M = indep_of_bases (bases_of_indep M) :=
 suffices M.indep = (indep_of_bases $ bases_of_indep M).indep, from eq_of_indep_eq this,
-by simp [indep_of_bases, bases_of_indep, indep_indep_of_bases, is_basis, ext, bases_bases_of_indep];
-exact λ I, iff.intro (λ hI, ⟨mem_powerset.mp $ mem_of_subset M.indep_subset_powerset_ground hI,
-  exists.elim (exists_basis_containing_indep hI) $ λ B hB, by unfold is_basis at hB;
+by { simp only [indep_of_bases, bases_of_indep, indep_indep_of_bases, is_basis,
+  ext, bases_bases_of_indep, mem_filter, mem_powerset, exists_prop],
+  exact λ I, iff.intro (λ hI, ⟨mem_powerset.mp $ mem_of_subset M.indep_subset_powerset_ground hI,
+  exists.elim (exists_basis_containing_indep hI) $ λ B hB, by { unfold is_basis at hB,
     exact exists.intro B ⟨⟨mem_powerset.1 $ mem_of_subset M.indep_subset_powerset_ground hB.2.1,
-      hB.2⟩, hB.1⟩⟩) $ λ hI, exists.elim hI.2 $ λ B hB, M.indep_of_subset_indep hB.1.2.1 hB.2
+      hB.2⟩, hB.1⟩ }⟩) $ λ hI, exists.elim hI.2 $ λ B hB, M.indep_of_subset_indep hB.1.2.1 hB.2 }
 
 /-- Corollary 1.2.6 -/
 theorem existsu_fund_circ_of_basis {m : indep E} {B : finset α} (hB : is_basis B m) {e : α}
   (he : e ∈ E \ B) : ∃ C, C ∈ circuits_circ_of_indep m ∧ C ⊆ insert e B ∧
   ∀ C' ∈ circuits_circ_of_indep m, C' ⊆ insert e B → C' = C :=
 begin
-  unfold is_basis at hB, simp at he,
+  unfold is_basis at hB, rw mem_sdiff at he,
   have : insert e B ∉ m.indep := hB.2 (insert e B) (insert_subset.mpr ⟨he.1,
     mem_powerset.mp $ mem_of_subset m.indep_subset_powerset_ground hB.1⟩) (ssubset_insert he.2),
   replace := existsu_circuit_of_dep_of_insert_indep hB.1 he.1 this,
@@ -786,16 +824,17 @@ def indep_of_restriction (m : indep E) {X : finset α} (hXE : X ⊆ E) : finset 
 
 def restriction (m : indep E) {X : finset α} (hXE : X ⊆ E) : indep X :=
 ⟨indep_of_restriction m hXE,
-by simp [indep_of_restriction, subset_iff],
-by simp [indep_of_restriction, m.empty_mem_indep],
-by unfold indep_of_restriction; exact λ x y hx hy, mem_filter.mpr
-  ⟨m.indep_of_subset_indep (mem_filter.mp hx).1 hy, subset.trans hy (mem_filter.mp hx).2⟩,
-by unfold indep_of_restriction; exact λ x y hx hy hcard,
+by simp only [indep_of_restriction, subset_iff, and_imp, imp_self,
+  mem_powerset, mem_filter, forall_true_iff],
+by simp only [indep_of_restriction, m.empty_mem_indep, empty_subset, and_self, mem_filter],
+by { unfold indep_of_restriction, exact λ x y hx hy, mem_filter.mpr
+  ⟨m.indep_of_subset_indep (mem_filter.mp hx).1 hy, subset.trans hy (mem_filter.mp hx).2⟩ },
+by { unfold indep_of_restriction, exact λ x y hx hy hcard,
   have hxm : x ∈ m.indep := (mem_filter.mp hx).1, have hym : y ∈ m.indep := (mem_filter.mp hy).1,
   have hxX : x ⊆ X := (mem_filter.mp hx).2, have hyX : y ⊆ X := (mem_filter.mp hy).2,
   have H : _ := m.indep_exch hxm hym hcard,
   let ⟨e, H, h₁⟩ := H in
-    ⟨e, H, mem_filter.mpr ⟨h₁, insert_subset.mpr ⟨mem_of_subset hyX (mem_sdiff.mp H).1, hxX⟩⟩⟩⟩
+    ⟨e, H, mem_filter.mpr ⟨h₁, insert_subset.mpr ⟨mem_of_subset hyX (mem_sdiff.mp H).1, hxX⟩⟩⟩ }⟩
 
 def deletion (m : indep E) {X : finset α} (hXE : X ⊆ E) : indep (E \ X) :=
 restriction m $ sdiff_subset E X
@@ -805,16 +844,18 @@ notation m `\` hxe := deletion m hxe
 
 lemma restriction_subset_restriction {X : finset α} (hX : X ⊆ E) (m : indep E) :
   (m ¦ hX).indep ⊆ m.indep :=
-by simp [restriction, indep_of_restriction, subset_iff]; exact λ _ hX'I _, hX'I
+by { simp only [restriction, indep_of_restriction, subset_iff, and_imp,
+  filter_congr_decidable, mem_filter],
+  exact λ _ hX'I _, hX'I }
 
 lemma restriction_trans {X Y : finset α} (hXY : X ⊆ Y) (hY : Y ⊆ E) (m : indep E) :
   (m ¦ subset.trans hXY hY) = ((m ¦ hY) ¦ hXY) :=
-by simp [restriction, indep_of_restriction, ext];
-exact λ I, iff.intro (λ h, ⟨⟨h.1, subset.trans h.2 hXY⟩, h.2⟩) $ λ h, ⟨h.1.1, h.2⟩
+by { simp only [restriction, indep_of_restriction, ext, mem_filter],
+  exact λ I, iff.intro (λ h, ⟨⟨h.1, subset.trans h.2 hXY⟩, h.2⟩) $ λ h, ⟨h.1.1, h.2⟩ }
 
 lemma subset_restriction_indep {X Y : finset α} {m : indep E} (hX : X ∈ m.indep) (hXY : X ⊆ Y)
   (hY : Y ⊆ E) : X ∈ (m ¦ hY).indep :=
-by simp [restriction, indep_of_restriction]; exact ⟨hX, hXY⟩
+by { simp only [restriction, indep_of_restriction, mem_filter], exact ⟨hX, hXY⟩ }
 
 /-def spans (X : finset α) {Y : finset α} (hY : Y ⊆ E) (m : indep E) : Prop :=
 X ∈ bases_bases_of_indep (m ¦ hY)-/
@@ -849,12 +890,13 @@ lemma R2_of_indep (m : indep E) {X Y : finset α} (hXY : X ⊆ Y) (hYE : Y ⊆ E
   𝓇 (subset.trans hXY hYE) m ≤ 𝓇 hYE m :=
 let hXE : X ⊆ E := subset.trans hXY hYE in let bX := 𝔹 hXE m in let bY := 𝔹 hYE m in
 have bXs : _ := 𝔹ₛ hXE m, have bYs : _ := 𝔹ₛ hYE m,
-by simp [bases_bases_of_indep] at bXs bYs; unfold rank_of_subset;
-have hBX : bX ∈ (m ¦ hYE).indep := mem_of_subset (restriction_subset_restriction hXY (m ¦ hYE))
-  ((restriction_trans hXY hYE m) ▸ bXs.2.1);
-exact exists.elim (exists_basis_containing_indep hBX) (λ B hB, calc
-  card bX ≤ card B : card_le_of_subset hB.1
-  ... = card bY : bases_of_indep_card_eq hB.2 bYs.2)
+by { simp only [bases_bases_of_indep, mem_powerset, filter_congr_decidable, mem_filter] at bXs bYs,
+  unfold rank_of_subset,
+  have hBX : bX ∈ (m ¦ hYE).indep := mem_of_subset (restriction_subset_restriction hXY (m ¦ hYE))
+    ((restriction_trans hXY hYE m) ▸ bXs.2.1),
+  exact exists.elim (exists_basis_containing_indep hBX) (λ B hB, calc
+    card bX ≤ card B : card_le_of_subset hB.1
+    ... = card bY : bases_of_indep_card_eq hB.2 bYs.2) }
 
 /-- Lemma 1.3.1 -/
 lemma R3_of_indep (m : indep E) {X Y : finset α} (hX : X ⊆ E) (hY : Y ⊆ E) :
@@ -872,15 +914,16 @@ begin
   unfold rank_of_subset,
   have bXuYs := 𝔹ₛ hXuY m, have bXiYs := 𝔹ₛ hXiY m,
   have bXs := 𝔹ₛ hX m, have bYs := 𝔹ₛ hY m,
-  simp [bases_bases_of_indep] at bXuYs bXiYs bXs bYs,
-  have rXiY : 𝓇 hXiY m = card bXiY := by simp [rank_of_subset],
+  simp only [bases_bases_of_indep, mem_powerset, filter_congr_decidable, mem_filter]
+    at bXuYs bXiYs bXs bYs,
+  have rXiY : 𝓇 hXiY m = card bXiY := by simp only [rank_of_subset],
   have hiu : X ∩ Y ⊆ X ∪ Y := subset.trans hXiYX hXXuY,
   have hbXiY : bXiY ∈ (m ¦ hXuY).indep := mem_of_subset
     (restriction_subset_restriction hiu (m ¦ hXuY)) ((restriction_trans hiu hXuY m) ▸ bXiYs.2.1),
   have HbbXiY := exists_basis_containing_indep hbXiY,
   exact exists.elim HbbXiY (by { intros B hB,
-    have rXuY : 𝓇 hXuY m = card B := by simp [rank_of_subset];
-      exact bases_of_indep_card_eq bXuYs.2 hB.2,
+    have rXuY : 𝓇 hXuY m = card B := by { simp only [rank_of_subset],
+      exact bases_of_indep_card_eq bXuYs.2 hB.2 },
     have hBXuY : B ⊆ X ∪ Y := mem_powerset.mp ((m ¦ hXuY).indep_subset_powerset_ground hB.2.1),
     have hBX : B ∩ X ∈ (m ¦ hX).indep := have hsub : _ := restriction_trans hXXuY hXuY m,
       have hBX : _ := ((m ¦ hXuY).indep_of_subset_indep hB.2.1 $ @inter_subset_left _ _ B X),
@@ -888,11 +931,12 @@ begin
     have hBY : B ∩ Y ∈ (m ¦ hY).indep := have hsub : _ := restriction_trans hYXuY hXuY m,
       have hBY : _ := ((m ¦ hXuY).indep_of_subset_indep hB.2.1 $ @inter_subset_left _ _ B Y),
       hsub.symm ▸ (subset_restriction_indep hBY (@inter_subset_right _ _ B Y) hYXuY),
-    have hBXr : card (B ∩ X) ≤ 𝓇 hX m := by unfold rank_of_subset;
-      exact card_of_indep_le_card_basis hBX bXs.2,
-    have hBYr : card (B ∩ Y) ≤ 𝓇 hY m := by unfold rank_of_subset;
-      exact card_of_indep_le_card_basis hBY bYs.2,
-    have hinter : (B ∩ X) ∩ (B ∩ Y) = B ∩ X ∩ Y := by simp,
+    have hBXr : card (B ∩ X) ≤ 𝓇 hX m := by { unfold rank_of_subset,
+      exact card_of_indep_le_card_basis hBX bXs.2 },
+    have hBYr : card (B ∩ Y) ≤ 𝓇 hY m := by { unfold rank_of_subset,
+      exact card_of_indep_le_card_basis hBY bYs.2 },
+    have hinter : (B ∩ X) ∩ (B ∩ Y) = B ∩ X ∩ Y := by simp only [finset.inter_assoc,
+      inter_right_comm, inter_self, inter_comm, inter_left_comm],
     have hBXiY : B ∩ X ∩ Y = bXiY :=
       by { have hsub : B ∩ X ∩ Y ⊆ bXiY :=
         by { by_contra h,
@@ -907,7 +951,7 @@ begin
           exact bXiYs.2.2 (insert a bXiY) hbXiYsubXiY this hindep }) },
       have hsuper : bXiY ⊆ B ∩ X ∩ Y :=
         by { rw [inter_assoc],
-        have := inter_subset_inter_of_subset hB.1 (X ∩ Y),
+        have := inter_subset_inter_right hB.1,
         have h : bXiY ∩ (X ∩ Y) = bXiY := inter_of_subset bXiYs.1,
         exact h ▸ this },
       exact subset.antisymm hsub hsuper },
@@ -935,7 +979,8 @@ variable [encodable α]
 
 def rank_of_indep (m : indep E) : rank E :=
 ⟨λ X hX, rank_of_subset hX m,
-λ X hX, ⟨dec_trivial, (by { have := basis_of_subset_spec hX m, simp [bases_bases_of_indep] at this,
+λ X hX, ⟨dec_trivial, (by { have := basis_of_subset_spec hX m,
+  simp only [bases_bases_of_indep, mem_powerset, filter_congr_decidable, mem_filter] at this,
   exact card_le_of_subset this.1 })⟩,
 λ X Y hXY hY, R2_of_indep m hXY hY,
 λ X Y hX hY, R3_of_indep m hX hY⟩
@@ -952,34 +997,37 @@ r (union_subset hX hY) + r (subset.trans (@inter_subset_left _ _ X Y) hX) ≤ r 
 
 lemma congr_for_rank (rk : rank_R2_R3 E ) {X Y : finset α} (hX : X ⊆ E) (hY : Y ⊆ E) (h : X = Y) :
 rk.r hX = rk.r hY :=
-by congr; exact h
+by { congr, exact h }
 
 -- Lemma 1.3.3
 lemma rank_union_lemma (rk : rank_R2_R3 E) {X Y : finset α} (hX : X ⊆ E) (hY : Y ⊆ E)
-  (hy : ∀ y, ∀ (h : y ∈ Y \ X), rk.r (by { simp at h,
+  (hy : ∀ y, ∀ (h : y ∈ Y \ X), rk.r (by { rw mem_sdiff at h,
     exact insert_subset.mpr ⟨mem_of_subset hY h.1, hX⟩ }) = rk.r hX) :
   rk.r (union_subset hX hY) = rk.r hX :=
 begin
   have hXuY : X ∪ Y ⊆ E := union_subset hX hY,
   induction h : (Y \ X) using finset.induction with a S ha ih generalizing X Y,
-  { congr, have H := congr_arg (λ x, X ∪ x) h, simp at H,
-    exact (union_eq_union_sdiff X Y).symm ▸ H },
+  { congr, have H := congr_arg (λ x, X ∪ x) h,
+    simp only [union_sdiff_self_eq_union, union_empty] at H, exact H },
   { have h₁ : rk.r hX + rk.r hX ≥ rk.r hXuY + rk.r hX :=
     by { have haa : a ∈ Y \ X := h.substr (mem_insert_self a S),
     have haX : insert a X ⊆ E := insert_subset.mpr ⟨mem_of_subset hY (mem_sdiff.mp haa).1, hX⟩,
     have hins : insert a S ⊆ E := h ▸ subset.trans (sdiff_subset Y X) hY,
     have hS : S ⊆ E := subset.trans (subset_insert a S) hins,
     have hXS : X ∪ S ⊆ E := union_subset hX hS,
-    have hrins : rk.r haX = rk.r hX := hy a haa, simp at haa,
+    have hrins : rk.r haX = rk.r hX := hy a haa, rw mem_sdiff at haa,
     have hrS : rk.r hXS = rk.r hX := by {
-      exact ih hX hS (by { intros y Hy, have : y ∈ Y \ X := by { simp at Hy,
-        simp [ext] at h, exact mem_sdiff.mpr ((h y).mpr $ or.inr Hy.1) }, exact hy y this })
-        hXS (by simp [ext] at h ⊢; exact λ y, iff.intro (λ Hy, Hy.1)
-        $ λ Hy, ⟨Hy, ((h y).mpr $ or.inr Hy).2⟩) },
+      exact ih hX hS (by { intros y Hy, have : y ∈ Y \ X := by { rw mem_sdiff at Hy,
+        simp only [ext, mem_insert, mem_sdiff] at h,
+        exact mem_sdiff.mpr ((h y).mpr $ or.inr Hy.1) }, exact hy y this })
+        hXS (by { simp only [ext, mem_insert, mem_sdiff] at h ⊢,
+          exact λ y, iff.intro (λ Hy, Hy.1) $ λ Hy, ⟨Hy, ((h y).mpr $ or.inr Hy).2⟩ }) },
     have hXuSiaX : (X ∪ S) ∩ insert a X ⊆ E := (subset.trans (@inter_subset_right _ _ (X ∪ S)
       (insert a X)) haX),
     have hr₁ : rk.r (union_subset hXS haX) = rk.r hXuY :=
-      by { exact congr_for_rank rk (union_subset hXS haX) hXuY (by simp [ext] at h ⊢;
+      by { exact congr_for_rank rk (union_subset hXS haX) hXuY (by {
+        simp only [ext, mem_union, union_comm, mem_insert, mem_sdiff, union_insert,
+          union_self, union_assoc] at h ⊢,
       exact λ x, iff.intro (λ hx, or.elim hx (λ hxa, or.inr $ hxa.substr haa.1) $
         λ H, or.elim H (by { intro hxS, exact or.inr ((h x).mpr $ or.inr hxS).1}) $
           by {exact (λ hxX, or.inl hxX) }) $
@@ -987,10 +1035,11 @@ begin
           by { intro hxY, by_cases hxX : x ∈ X,
             { exact or.inr (or.inr hxX) },
             { exact or.elim ((h x).mp ⟨hxY, hxX⟩) (λ H, or.inl H)
-              (λ HS, or.inr $ or.inl HS) } }) },
-    have hr₂ : rk.r hXuSiaX = rk.r hX := by congr; simp [ext];
+              (λ HS, or.inr $ or.inl HS) } } }) },
+    have hr₂ : rk.r hXuSiaX = rk.r hX := by { congr,
+      simp only [ext, mem_union, union_comm, mem_insert, mem_inter],
       exact λ x, iff.intro (λ hx, or.elim hx.1 (or.elim hx.2
-        (λ H₁ H₂, false.elim $ ha $ H₁.subst H₂) $ λ h _, h) id) (λ hx, ⟨or.inr hx, or.inr hx⟩),
+        (λ H₁ H₂, false.elim $ ha $ H₁.subst H₂) $ λ h _, h) id) (λ hx, ⟨or.inr hx, or.inr hx⟩) },
     calc rk.r hX + rk.r hX = rk.r hXS + rk.r haX : by rw [hrS, hrins]
     ... ≥ rk.r (union_subset hXS haX) + rk.r hXuSiaX : rk.submodular (union_subset hX hS) haX
     ... = _ : by rw [hr₁, hr₂] },
